Cvc/Proto2/Untyped/BVar.lean
@@ -25,26 +25,48 @@ def BVar := Term
 /-- An array of bound variables. -/
 abbrev BVars := Array BVar
 
-namespace Term
+namespace BVar
 
 /-- A bound variable of the given sort.
 
 Only meaningful under a binder: the bound variables of a definition's body, or of a quantifier,
 lambda or witness. Each call produces a fresh variable even for the same name and sort.
 -/
-def mkBVar (srt : Srt) (name : String) : Env BVar :=
-  runUnsafe fun tm => tm.mkVar srt.toUnsafe name
-
-end Term
-
-namespace BVar
-
-@[inherit_doc Term.mkBVar]
-def mk (srt : Srt) (name : String) : Env BVar := Term.mkBVar srt name
+def mk (srt : Srt) (name : String) : Env BVar := runUnsafe fun tm => tm.mkVar srt.toUnsafe name
 
 /-- Turns itself into a term. -/
 def toTerm : (bv : BVar) → Term := id
 
+/-- Creates a lambda from a bound variables and a body. -/
+def lambda (bv : BVar) (body : Term) : Env Term := runUnsafe fun tm => do
+  let bvs ← tm.mkTerm .VARIABLE_LIST #[bv]
+  tm.mkTerm .LAMBDA #[bvs, body]
+
 instance : Coe BVar Term := ⟨toTerm⟩
 
 end BVar
+
+namespace BVars
+
+/-- Turns itself into a *variable list* term, used to create `Term.lambda`s. -/
+def toTerm (bvs : BVars) : Env Term := runUnsafe fun tm => tm.mkTerm .VARIABLE_LIST bvs
+
+/-- Creates a lambda from some bound variables and a body. -/
+def lambda (bvs : BVars) (body : Term) : Env Term := do
+  let bvs ← bvs.toTerm
+  runUnsafe fun tm => tm.mkTerm .LAMBDA #[bvs, body]
+
+end BVars
+
+namespace Term
+
+@[inherit_doc BVar.mk]
+def mkBVar (srt : Srt) (name : String) : Env BVar := BVar.mk srt name
+
+@[inherit_doc BVars.lambda]
+def lambda (bvs : BVars) (body : Term) : Env Term := bvs.lambda body
+
+@[inherit_doc BVar.lambda]
+def lambda1 (bv : BVar) (body : Term) : Env Term := bv.lambda body
+
+end Term
