Cvc/Proto2/Typed/Symbols.lean
@@ -35,7 +35,8 @@ end Sig
 end Symbols
 
 class Symbols (S : Symbols.Sig) where
-  idents : S.Idents
+  InitData : Type := Unit
+  idents : InitData → S.Idents
   mapM {W W' : Symbols.Wrap} [Monad m]
     (s : S W) (f : {α : Type} → [ToTyp α] → [TermToValue α] → W α → m (W' α)) : m (S W')
 
@@ -44,7 +45,7 @@ section variable {S : Symbols.Sig} [inst : Symbols S]
 namespace Symbols
 
 namespace Sig
-abbrev idents : S.Idents := inst.idents
+abbrev idents : inst.InitData → S.Idents := inst.idents
 abbrev Idents.get := @Sig.idents
 
 abbrev mapM := @inst.mapM
@@ -76,13 +77,11 @@ end
 
 
 
-
-/-! ## Example
+/-! ## Example 1
 
 The code below is an example of the user experience for the `Symbols` API.
 -/
-
-
+namespace Ex1
 
 /-- User-defined symbol structure. -/
 structure MySymbols (W : Symbols.Wrap) : Type where
@@ -92,16 +91,6 @@ structure MySymbols (W : Symbols.Wrap) : Type where
 
 namespace MySymbols
 
-/-- `Symbols` instance giving access to the `Symbols` API. -/
-instance : Symbols MySymbols where
-  idents := { myBoolVar := "myBoolVar", myIntVar := "myIntVar", myRealVar := "myRealVar" }
-  mapM syms f := do
-    return {
-      myBoolVar := ← f syms.myBoolVar
-      myIntVar := ← f syms.myIntVar
-      myRealVar := ← f syms.myRealVar
-    }
-
 /-- Idents alias. -/
 abbrev Idents := Symbols.Sig.Idents MySymbols
 
@@ -110,6 +99,15 @@ abbrev Terms := Symbols.Sig.Terms MySymbols
 
 /-- Values alias. -/
 abbrev Values := Symbols.Sig.Values MySymbols
+
+/-- `Symbols` instance giving access to the `Symbols` API. -/
+instance : Symbols MySymbols where
+  idents _ := { myBoolVar := "myBoolVar", myIntVar := "myIntVar", myRealVar := "myRealVar" }
+  mapM syms f := return {
+    myBoolVar := ← f syms.myBoolVar
+    myIntVar := ← f syms.myIntVar
+    myRealVar := ← f syms.myRealVar
+  }
 
 /-! With this instance users can very easily declare or get-value their symbols. -/
 
@@ -124,3 +122,44 @@ def findCex (syms : MySymbols.Terms) (solver : Solver)
   solver.checkSat? assuming (ifSat := syms.getValues solver)
 
 end MySymbols
+
+end Ex1
+
+
+
+/-! ## Example 2 -/
+namespace Ex2
+
+structure MySymbols (W : Symbols.Wrap) where
+  boolVars : Array (W Bool)
+  intVars : Array (W Int)
+  realVars : Array (W Rat)
+
+namespace MySymbols
+
+abbrev Idents := Symbols.Sig.Idents MySymbols
+abbrev Terms := Symbols.Sig.Terms MySymbols
+abbrev Values := Symbols.Sig.Values MySymbols
+
+instance : Symbols MySymbols where
+  InitData := Idents
+  idents := id
+  mapM symbols f := return {
+    boolVars := ← symbols.boolVars.mapM f
+    intVars := ← symbols.intVars.mapM f
+    realVars := ← symbols.realVars.mapM f
+  }
+
+/-- Declares `MySymbols` in `solver` -/
+def declare (idents : MySymbols.Idents) : Env MySymbols.Terms :=
+  idents.declare
+
+/-- Tries to extract a satisfiable `MySymbols`-assignment in `solver`. -/
+def findCex (syms : MySymbols.Terms) (solver : Solver)
+  (assuming : Option (Typed.Terms Bool) := none)
+: Env (Option MySymbols.Values) :=
+  solver.checkSat? assuming (ifSat := syms.getValues solver)
+
+end MySymbols
+
+end Ex2
